abstract machine corrections

abstract_machine/abstract_machine.v
@@ -13,13 +13,11 @@ Module Type ABSTRACT_MACHINE.
   (value         : Set)
 
   (load          : term -> configuration)
-  (value_to_conf : value -> configuration)
   (final         : configuration -> option value)
   (transition    : configuration -> configuration -> Prop)
   (next_conf     : entropy -> configuration -> option configuration).
 
-  Coercion value_to_conf : value >-> configuration.
-
+  Definition is_final c := exists v, final c = Some v.
 
   Instance rws : REWRITING_SYSTEM configuration :=
   { transition := transition }.
@@ -29,9 +27,7 @@ Module Type ABSTRACT_MACHINE.
   (final_correct :                                                              forall c,
        final c <> None -> ~exists c', c → c')
   (trans_computable :                                                       forall c1 c2,
-       c1 → c2 <-> exists e, next_conf e c1 = Some c2)
-  (finals_are_vals :                                                          forall c v,
-       final c = Some v <-> c = v).
+       c1 → c2 <-> exists e, next_conf e c1 = Some c2).
 
 
 
@@ -40,7 +36,7 @@ Module Type ABSTRACT_MACHINE.
       preservation :                                                        forall c1 c2,
           P c1  ->  c1 → c2  ->  P c2;
       progress :                                                               forall c1,
-          P c1  ->  (exists (v : value), c1 = v) \/ (exists c2, c1 → c2)
+          P c1  ->  (is_final c1) \/ (exists c2, c1 → c2)
   }.
 
 End ABSTRACT_MACHINE.
