refocusing_examples/miniml_check.v
@@ -319,27 +319,20 @@ Module MiniML_HandMachine <: ABSTRACT_MACHINE.
   Qed.
 
 
-  Fact finals_are_vals :                                                     forall st v,
-       final st = Some v <-> st = v. 
-
-  Proof. exact MiniML_EAM.finals_are_vals. Qed.
+  Class SafeRegion (P : configuration -> Prop) :=
+  {
+      preservation :                                                      forall st1 st2,
+          P st1  ->  st1 → st2  ->  P st2;
+      progress :                                                              forall st1,
+          P st1  ->  is_final st1 \/ (exists st2, st1 → st2)
+  }.
 
 
   Definition term          := term.
   Definition value         := value init_ckind.
   Definition configuration := configuration.
   Definition load          := load.
-  Definition value_to_conf : value ->  configuration := value_to_conf.
-  Coercion   value_to_conf : value >-> configuration.
   Definition final         := final.
-
-
-  Class SafeRegion (P : configuration -> Prop) :=
-  { 
-      preservation :                                                        forall t1 t2,
-          P t1  ->  t1 → t2  ->  P t2;
-      progress :                                                               forall t1,
-          P t1  ->  (exists (v : value), t1 = v) \/ (exists t2, t1 → t2)
-  }.
+  Definition is_final c := exists v, final c = Some v.
 
 End MiniML_HandMachine.
